Refactoring

multi_actris/examples/mpc.v
@@ -7,6 +7,57 @@ Notation B := 1.
 Notation C := 2.
 Notation D := 3.
 
+Definition A_prog : val :=
+  λ: "ch",
+     let: "a" := #42 in
+     let: "a1" := #10 in
+     let: "a2" := #20 in
+     let: "a3" := #12 in
+     send "ch" #B "a2";;
+     send "ch" #C "a3";;
+     let: "b1" := recv "ch" #B in
+     let: "c1" := recv "ch" #C in
+     let: "s1" := "a1"+"b1"+"c1" in
+     send "ch" #B "s1";;
+     send "ch" #C "s1";;
+     let: "s2" := recv "ch" #B in
+     let: "s3" := recv "ch" #C in
+     send "ch" #D ("s1"+"s2"+"s3").
+
+Definition B_prog : val :=
+  λ: "ch",
+     let: "b" := #100 in
+     let: "b1" := #20 in
+     let: "b2" := #30 in
+     let: "b3" := #50 in
+     let: "a2" := recv "ch" #A in
+     send "ch" #A "b1";;
+     send "ch" #C "b3";;
+     let: "c2" := recv "ch" #C in
+     let: "s1" := recv "ch" #A in
+     let: "s2" := "a2"+"b2"+"c2" in
+     send "ch" #A "s2";;
+     send "ch" #C "s2";;
+     let: "s3" := recv "ch" #C in
+     send "ch" #D ("s1"+"s2"+"s3").
+
+Definition C_prog : val :=
+  λ: "ch",
+     let: "c" := #7 in
+     let: "c1" := #1 in
+     let: "c2" := #2 in
+     let: "c3" := #4 in
+     let: "a3" := recv "ch" #A in
+     send "ch" #A "c1";;
+     let: "b3" := recv "ch" #B in
+     send "ch" #B "c2";;
+     let: "s1" := recv "ch" #A in
+     let: "s3" := "a3"+"b3"+"c3" in
+     send "ch" #A "s3";;
+     let: "s2" := recv "ch" #B in
+     send "ch" #B "s3";;
+     send "ch" #D ("s1"+"s2"+"s3").
+
 Definition program : val :=
   λ: <>,
      let: "cs" := new_chan #4 in
@@ -14,65 +65,9 @@ Definition program : val :=
      let: "ch1" := get_chan "cs" #B in
      let: "ch2" := get_chan "cs" #C in
      let: "ch3" := get_chan "cs" #D in
-     (* A *)
-     Fork (let: "a" := #42 in
-           let: "a1" := #10 in
-           let: "a2" := #20 in
-           let: "a3" := #12 in
-           (* (<(Send,B) @ (a2:Z)> MSG #a2 ; <(Send,C) @ (a3:Z)> MSG #a3 ; *)
-           send "ch0" #B "a2";;
-           send "ch0" #C "a3";;
-           (* <(Recv,B) @ (b1:Z)> MSG #b1 ; <(Recv,C) @ (c1:Z)> MSG #c1 ; *)
-           let: "b1" := recv "ch0" #B in
-           let: "c1" := recv "ch0" #C in
-           (* <(Send,B) @ (s1:Z) (a1:Z)> MSG #s1 {{ ⌜(s1 = a1 + b1 + c1)%Z⌝ }} ; *)
-           let: "s1" := "a1"+"b1"+"c1" in
-           send "ch0" #B "s1";;
-           (* <(Send,C)> MSG #s1 ; *)
-           send "ch0" #C "s1";;
-           (* <(Recv,B) @ (s2:Z)> MSG #s2 ; <(Recv,C) @ (s3:Z)> MSG #s3; *)
-           let: "s2" := recv "ch0" #B in
-           let: "s3" := recv "ch0" #C in
-           send "ch0" #D ("s1"+"s2"+"s3"));;
-     (* B *)
-     Fork (let: "b" := #100 in
-           let: "b1" := #20 in
-           let: "b2" := #30 in
-           let: "b3" := #50 in
-           (* <(Recv,A) @ (a2:Z)> MSG #a2 ; <(Send,A) @ (b1:Z)> MSG #b1 ; *)     
-           let: "a2" := recv "ch1" #A in
-           send "ch1" #A "b1";;
-           (* <(Send,C) @ (b3:Z)> MSG #b3 ; <(Recv,C) @ (c2:Z)> MSG #c2 ; *)
-           send "ch1" #C "b3";;
-           let: "c2" := recv "ch1" #C in
-           (* <(Recv,A) @ (s1:Z)> MSG #s1 ; *)
-           let: "s1" := recv "ch1" #A in
-           (* <(Send,A) @ (s2:Z) (b2:Z)> MSG #s2 {{ ⌜(s2 = a2 + b2 + c2)%Z⌝ }} ; *)
-           let: "s2" := "a2"+"b2"+"c2" in
-           send "ch1" #A "s2";;
-           (* <(Send,C)> MSG #s2 ; <(Recv,C) @ (s3:Z)> MSG #s3 ; *)
-           send "ch1" #C "s2";;
-           let: "s3" := recv "ch1" #C in
-           send "ch1" #D ("s1"+"s2"+"s3"));;
-     Fork (let: "c" := #7 in
-           let: "c1" := #1 in
-           let: "c2" := #2 in
-           let: "c3" := #4 in
-           (* <(Recv,A) @ (a3:Z)> MSG #a3 ; <(Send,A) @ (c1:Z)> MSG #c1 ; *)
-           let: "a3" := recv "ch2" #A in
-           send "ch2" #A "c1";;
-           (* <(Recv,B) @ (b3:Z)> MSG #b3 ; <(Send,B) @ (c2:Z)> MSG #c2 ; *)
-           let: "b3" := recv "ch2" #B in
-           send "ch2" #B "c2";;
-           (* <(Recv,A) @ (s1:Z)> MSG #s1 ; *)
-           let: "s1" := recv "ch2" #A in
-           (* <(Send,A) @ (s3:Z) (c3:Z)> MSG #s3 {{ ⌜(s3 = a3 + b3 + c3)%Z⌝ }} ; *)
-           let: "s3" := "a3"+"b3"+"c3" in
-           send "ch2" #A "s3";;
-           (* <(Recv,B) @ (s2:Z)> MSG #s2 ; <(Send,B)> MSG #s3; *)
-           let: "s2" := recv "ch2" #B in
-           send "ch2" #B "s3";;
-           send "ch2" #D ("s1"+"s2"+"s3"));;
+     Fork (A_prog "ch0");;
+     Fork (B_prog "ch1");;
+     Fork (C_prog "ch2");;
      let: "res1" := recv "ch3" #A in
      let: "res2" := recv "ch3" #B in
      let: "res3" := recv "ch3" #C in
@@ -82,6 +77,9 @@ Definition program : val :=
 Section mpc_protocols.
   Context `{!heapGS Σ, chanG Σ}.
 
+  Definition tail_prot (sum : Z) : iProto Σ :=
+     (<(Send,D)> MSG #sum ; END)%proto.
+
   Definition A_prot (p : Z → iProto Σ) : iProto Σ :=
     (<(Send,B) @ (a2:Z)> MSG #a2 ; <(Send,C) @ (a3:Z)> MSG #a3 ;
      <(Recv,B) @ (b1:Z)> MSG #b1 ; <(Recv,C) @ (c1:Z)> MSG #c1 ;
@@ -89,6 +87,10 @@ Section mpc_protocols.
      <(Send,C)> MSG #s1 ;
      <(Recv,B) @ (s2:Z)> MSG #s2 ; <(Recv,C) @ (s3:Z)> MSG #s3;
      p (s1 + s2 + s3)%Z)%proto.
+
+  Lemma A_spec c :
+    {{{ c ↣ A_prot tail_prot }}} A_prog c {{{ RET #(); True }}}.
+  Proof. iIntros (Φ) "Hc HΦ". wp_lam. wp_chan_pures. by iApply "HΦ". Qed.
 
   Definition B_prot (p : Z → iProto Σ) : iProto Σ :=
     (<(Recv,A) @ (a2:Z)> MSG #a2 ; <(Send,A) @ (b1:Z)> MSG #b1 ;
@@ -98,6 +100,10 @@ Section mpc_protocols.
      <(Send,C)> MSG #s2 ; <(Recv,C) @ (s3:Z)> MSG #s3 ;
      p (s1 + s2 + s3)%Z)%proto.
 
+  Lemma B_spec c :
+    {{{ c ↣ B_prot tail_prot }}} B_prog c {{{ RET #(); True }}}.
+  Proof. iIntros (Φ) "Hc HΦ". wp_lam. wp_chan_pures. by iApply "HΦ". Qed.
+
   Definition C_prot (p : Z → iProto Σ) : iProto Σ :=
     (<(Recv,A) @ (a3:Z)> MSG #a3 ; <(Send,A) @ (c1:Z)> MSG #c1 ;
      <(Recv,B) @ (b3:Z)> MSG #b3 ; <(Send,B) @ (c2:Z)> MSG #c2 ;
@@ -106,13 +112,14 @@ Section mpc_protocols.
      <(Recv,B) @ (s2:Z)> MSG #s2 ; <(Send,B)> MSG #s3;
      p (s1 + s2 + s3)%Z)%proto.
 
+  Lemma C_spec c :
+    {{{ c ↣ C_prot tail_prot }}} C_prog c {{{ RET #(); True }}}.
+  Proof. iIntros (Φ) "Hc HΦ". wp_lam. wp_chan_pures. by iApply "HΦ". Qed.
+
   Definition D_prot : iProto Σ :=
     (<(Recv,A) @ (sum : Z)> MSG #sum ;
      <(Recv,B)> MSG #sum;
      <(Recv,C)> MSG #sum; END)%proto.
-
-  Definition tail_prot (sum : Z) : iProto Σ :=
-     (<(Send,D)> MSG #sum ; END)%proto.
 
   Definition mpc_prot_pool : list (iProto Σ) :=
      [A_prot tail_prot; B_prot tail_prot; C_prot tail_prot; D_prot].
@@ -121,24 +128,18 @@ Section mpc_protocols.
     ⊢ iProto_consistent mpc_prot_pool.
   Proof. rewrite /mpc_prot_pool. iProto_consistent_take_steps. Qed.
 
-  (* TODO: Clean up and move to proofmode.v? *)
-  Tactic Notation "wp_recv" := try wp_recv (?) as "_"; try wp_recv as "_".
-  Tactic Notation "wp_send" := wp_send with "[//]".
-  Tactic Notation "wp_chan_pures" := repeat (repeat wp_send; repeat wp_recv).
-
   Lemma mpc_spec :
     {{{ True }}} program #() {{{ RET #(); True }}}.
   Proof.
-    iIntros (Φ) "_ HΦ".
-    wp_lam.
+    iIntros (Φ) "_ HΦ". wp_lam.
     wp_new_chan mpc_prot_pool with mpc_consistent
       as (ch0 ch1 ch2 ch3) "Hc0" "Hc1" "Hc2" "Hc3".
     wp_smart_apply (wp_fork with "[Hc0]").
-    { iIntros "!>". by wp_chan_pures. }
+    { by iApply (A_spec with "[$]"). }
     wp_smart_apply (wp_fork with "[Hc1]").
-    { iIntros "!>". by wp_chan_pures. }
+    { by iApply (B_spec with "[$]"). }
     wp_smart_apply (wp_fork with "[Hc2]").
-    { iIntros "!>". by wp_chan_pures. }
+    { by iApply (C_spec with "[$]"). }
     wp_chan_pures. wp_smart_apply wp_assert. wp_pures.
     iSplitR; [by case_bool_decide|]. iIntros "!>!>".
     wp_smart_apply wp_assert. wp_pures.
